compiler/wasm/wasm2LangScript.sml
@@ -46,6 +46,11 @@ Datatype: valtype
   | TExtRef
 End
 
+Datatype: global
+  = Gconst valtype
+  | Gmut   valtype
+End
+
 Type addrtype = “:width”
 
 Datatype: limits
@@ -54,6 +59,15 @@ Datatype: limits
 End
 
 Type memtyp = “:(addrtype # limits)”
+Type mem = “:word8 list”
+
+(* Type resulttype = “:[valtype]” *)
+Type functype = “:[valtype] # [valtype]”
+
+
+
+
+
 
 (* Note on style :
   instructions data constructors have their return types
@@ -461,30 +475,11 @@ End
   (*   Misc Notations/"types"   *)
   (******************************)
 
-Type t = “:valtype”
-Type functype = “:t list # t list”
-(* Datatype: functype
-  =
-  |
-End *)
-
-
-(* QQ these represent block types? *)
-Datatype:
-  tb = Tbf num (* | Tbv (t option) *)
-End
-
-(* Datatype: ctrlFlow_instr
-  | CtrlFlow  ctrlFlow_instr
-End *)
-
 Datatype: blocktype
   = BlkNil
   | BlkVal valtype
-  | BlkIdx num
+  | BlkIdx word32
 End
-
-(* TODO switch out nums in AST to index *)
 
 Datatype: instr
 
@@ -516,28 +511,27 @@ Datatype: instr
 
 End
 
-
-Datatype: func =
+(* Datatype: func =
   <|
-    name       : string     ;
-    type       : functype   ;
-    body       : instr list ;
-    localTypes : valtype list
+    name       : string      ;
+    type       : functype    ;
+    body       : instr   list;
+    localTypes : valtype list;
   |>
-End
+End *)
 
 (* MM: HOL doesn't have a utf8 library *)
 (* Datatype: module =
   <|
-  funcs   : func list
-  tables  : table list
-  mems    : mem list
-  globals : global list
-  elems   : elem list
-  datas   : data list
-  start   :
-  imports : import list
-  exports : export list
+    funcs   : func    list ;
+    (* tables  : table   list ; *)
+    mems    : mem     list ;
+    globals : global  list ;
+    (* elems   : elem    list ; *)
+    (* datas   : data    list ; *)
+    start   : index        ;
+    (* imports : import  list ; *)
+    (* exports : export  list ; *)
   |>
 End *)
 
